%SECTION: SETUP
% region: document class
\documentclass{article}

% endregion

% region: packages 
\usepackage{xr}
\usepackage{physics}
\usepackage{amsmath}
% \usepackage{float}
% \usepackage{tabularray}
% \UseTblrLibrary{booktabs}
% \usepackage[
%     backend=biber,
%     style=apa
% ]{biblatex}

% endregion

% region: title 
% Title
% \title{
%     dsds
% }
% \author{Cao Bittencourt}
% \date{\today}

% endregion

\pagestyle{empty}

%SECTION: PAPER
\begin{document}

\begin{gather}
    % \text{Interchangeability cannot be } I(s(\boldsymbol{a_k},\boldsymbol{a_k}) \text{because I is already the Identity Matrix.}
    % german character ß (esset, eszet, or sharp s) is itself interchangeable with 'ss'
    % thus ß could stand for sufficiently similar / sufficient similarity (ss)
    \boldsymbol{\Lambda} = (\Lambda_{1}, ..., \Lambda_{n}),\\
    % \Lambda_{k} = 
    %     \frac{
    %         \sum_{q=1}^{n}{
    %             \textit{\ss}_{k,q}
    %             w_q
    %             % \textit{\ss}(s(\boldsymbol{a_k},\boldsymbol{a_q}), \tau_k, \tau_q, c_q)
    %         }
    %     }{
    %         W
    %     },\\
    % \Lambda(\boldsymbol{\textbf{\textit{\ss}}_{k}}, \boldsymbol{w}) = 
    %     \frac{
    %         \sum_{q=1}^{n}{
    %             \textit{\ss}_{k,q}
    %             w_q
    %             % \textit{\ss}(s(\boldsymbol{a_k},\boldsymbol{a_q}), \tau_k, \tau_q, c_q)
    %         }
    %     }{
    %         W
    %     },\\
    \Lambda_k = 
    \Lambda(\boldsymbol{\textbf{\textit{\ss}}_{k}}, \boldsymbol{w}) = 
        % \left(
        \left(
            \frac{1}{W}
        \right)
        % \right)
        \sum_{q=1}^{n}{
            \textit{\ss}_{k,q}
            w_q
            % \textit{\ss}(s(\boldsymbol{a_k},\boldsymbol{a_q}), \tau_k, \tau_q, c_q)
        },\\
    \text{vs}_k = 
    \text{vs}(\boldsymbol{\textbf{\textit{\ss}}_{k}}, \boldsymbol{w}, \boldsymbol{y}) = 
    % \left(
    \left(
        \frac{1}{W}
    \right)
    % \right)
        \sum_{q=1}^{n}{
            \textit{\ss}_{q,k}
            w_q
            u(y_q,y_k)
        }
        ,\\
    \textit{\ss}_{k,q} = 
        \text{eq}(s(\boldsymbol{a_k},\boldsymbol{a_q}), c_q)\\
    u(y_q,y_k) =
    \begin{cases}
        1, \text{if } y_k \geq y_q.\\
        0, \text{otherwise.}
    \end{cases}\\
    % \textit{\ss}_{k,q} = 
    %     \text{eq}(s(\boldsymbol{a_k},\boldsymbol{a_q}), c_q)
    %     \times
    %     \text{eq}(\tau_k, \tau_q, c_q)\\
    W = 
        \sum_{q=1}^{n}{
            w_q
        }\\
    \textbf{\ss} = 
    % \textbf{SS} = 
    \begin{bmatrix}
        \textit{\ss}_{1,1} & \hdots & \textit{\ss}_{n,1}\\
        \vdots & \ddots & \vdots\\
        \textit{\ss}_{1,n} & \hdots & \textit{\ss}_{n,n}\\
    \end{bmatrix} = 
    % \textbf{\ss} = 
    % \textbf{SS} = 
    \begin{bmatrix}
        1 & \hdots & \textit{\ss}_{k,1} & \hdots & \textit{\ss}_{n,1}\\
        \vdots & \ddots & \vdots & \vdots & \vdots\\
        \textit{\ss}_{1,k} & \hdots & 1 & \hdots & \textit{\ss}_{n,k}\\
        \vdots & \vdots & \vdots & \ddots & \vdots\\
        \textit{\ss}_{1,n} & \hdots & \textit{\ss}_{k,n} & \hdots & 1\\
    \end{bmatrix}\\
    \boldsymbol{\textbf{\textit{\ss}}_{k}} = (\textit{\ss}_{k,1}, ..., \textit{\ss}_{k,n})\\
    \boldsymbol{\textbf{\textit{\ss}}_{q}} = (\textit{\ss}_{q,1}, ..., \textit{\ss}_{q,n})\\
    \gamma_{k} = 
    % \gamma(\boldsymbol{\tilde{a}_k}) = 
        \text{sq}(\boldsymbol{\tilde{a}_k})\\
    % c_{k} = 
    % c(\boldsymbol{a_k}, \gamma_{k}) = 
    %     \left( \frac{1}{m} \right)
    %     \sum_{i=1}^{m}{
    %         \text{eq}\left(
    %             \frac{
    %                 a_{i}^{k}
    %             }{
    %                 a_{\max}^{k}
    %             }, \gamma_{k}
    %             \right)
    %         }
    %         \times
    %         \tilde{a}_{i}^{k},\\
    % c_{k} = 
    % c(\boldsymbol{a_k}, \gamma_{k}) = 
    %     \left( \frac{1}{m} \right)
    %     \sum_{i=1}^{m}{
    %         % \theta_{i}^{k}
    %         % \"a_{i}^{k}
    %         % \overset{e}{a}_{i}^{k}
    %         % \"a_{i}^{k}
    %         % ә_{i}^{k}
    %         {\"a}_{i}^{k}
    %         \tilde{a}_{i}^{k}
    %         },\\
    c_{k} = 
    c(\boldsymbol{a_k}, \gamma_{k}) = 
    \frac{
        \sum_{i=1}^{m}{
            {\"a}_{i}^{k}
            \tilde{a}_{i}^{k}
            }
    }{
        \sum_{i=1}^{m}{
            {\"a}_{i}^{k}
            }
    },\\
    % \theta_{i}^{k} =
    {\"a}_{i}^{k} =
    % \theta(a_{i}^{k},a_{\max}^{k},\gamma_{k}) = 
    \text{eq}\left(
        \frac{
            a_{i}^{k}
        }{
            % \max_{j}{a_{j}^{k}}
            \max{a_{j}^{k}}
            % a_{\max}^{k}
        },
        \gamma_{k}
    \right)\\
    % \theta_{i}^{k} = \text{eq}(\tilde{a}_{i}^{k}, \gamma_{k})\\
    \boldsymbol{{\"a}_{k}} = ({\"a}_{1}^{k}, ..., {\"a}_{m}^{k})\\
    \boldsymbol{{\"a}_{q}} = ({\"a}_{1}^{q}, ..., {\"a}_{m}^{q})\\
    \boldsymbol{{\"a}_{n}} = ({\"a}_{1}^{n}, ..., {\"a}_{m}^{n})\\
    \textbf{{\"A}} = 
    \begin{bmatrix}
        {\"a}_{1}^{1} & \hdots & {\"a}_{m}^{1}\\
        \vdots & \ddots & \vdots\\
        {\"a}_{1}^{n} & \hdots & {\"a}_{m}^{n}\\
    \end{bmatrix}\\
    % \boldsymbol{\theta_{k}} = (\theta_{1}^{k}, ..., \theta_{m}^{k})\\
    % \boldsymbol{\theta_{q}} = (\theta_{1}^{q}, ..., \theta_{m}^{q})\\
    % \boldsymbol{\theta_{n}} = (\theta_{1}^{n}, ..., \theta_{m}^{n})\\
    % \boldsymbol{\Theta} = 
    % \begin{bmatrix}
    %     \theta_{1}^{1} & \hdots & \theta_{m}^{1}\\
    %     \vdots & \ddots & \vdots\\
    %     \theta_{1}^{n} & \hdots & \theta_{m}^{n}\\
    % \end{bmatrix}\\
    % \text{eq}(x,M,b) = 
    % x\left(
    %     1 + M (1 - x) \exp(-b(x - M))
    % \right) ^ {
    %     -\frac{
    %         1 - x
    %     }{
    %         1 - M
    %     }
    % }\\
    % \text{eq}(x,M,b) = 
    % x\left[
    %     1 + M (1 - x) \exp(-b(x - M))
    % \right] ^ {
    %     -\frac{
    %         1 - x
    %     }{
    %         1 - M
    %     }
    % }\\
    % \text{eq}(x,M,b) = 
    % x\left\{
    %     1 + M (1 - x) \exp[-b(x - M)]
    % \right\} ^ {
    %     -\frac{
    %         1 - x
    %     }{
    %         1 - M
    %     }
    % }, x, M \in [0,1]\\
    % \text{eq}(x,M) = 
    % x\left\{
    %     1 + M (1 - x) \exp[-
    %         % \tan\left[
    %         \tan \bigg(
    %             \frac{\pi}{2}
    %             % (\pi / 2)
    %             \cos\big(
    %                 x (1 - M)
    %             \big)
    %         \bigg)
    %         % \right]
    %         (x - M)
    %      ]
    % \right\} ^ {
    %     -\frac{
    %         1 - x
    %     }{
    %         1 - M
    %     }
    % },\\ x, M \in [0,1].\\
    % \text{eq}(x,M) = 
    % x\left\{
    %     1 + M (1 - x) \exp[-
    %         (x - M)
    %         \tan{\theta}
    %      ]
    % \right\} ^ {
    %     -\frac{
    %         1 - x
    %     }{
    %         1 - M
    %     }
    % },\\
    % \theta = 
    %     % \frac{\pi}{2}
    %     (\pi/2)
    %     [1 - x(1 - M)] ^ {x(1 - M)},\\
    % x, M \in [0,1].\\
    % \text{eq}(x,1,b) = 
    % x\left\{
    %     1 + 1 \times (1 - x) \exp[-b(x - 1)]
    % \right\} ^ {
    %     -\frac{
    %         1 - x
    %     }{
    %         1 - 1
    %     }
    % } = \\
    % x\left\{
    %     1 + (1 - x) \exp[-b(x - 1)]
    % \right\} ^ {
    %     -\frac{
    %         1 - x
    %     }{
    %         0
    %     }
    % } = \\
    % \begin{cases}
    %     0, \text{if } x \neq 1.\\
    %     1, \text{otherwise}.
    % \end{cases},
    % x \in [0,1]\\
    % \text{eq}(x,0,b) =
    % x\left\{
    %     1 + 0 \times (1 - x) \exp[-b(x - 0)]
    % \right\} ^ {
    %     -\frac{
    %         1 - x
    %     }{
    %         1 - 0
    %     }
    % } =
    % \frac{x}{1} = 
    % x\\
    % \text{eq}(x,M,b) = 
    % \frac{x}{
    %     \left(
    %     1 + M (1 - x) \exp(-b(x - M))
    % \right) ^ {
    %     \frac{
    %         1 - x
    %     }{
    %         1 - M
    %     }
    % }
    % }
    % \text{sq}(x,\sigma_x) = 
    % \frac{\sigma_x}{2} + 
    % \left(
    %     1 - \frac{\sigma_x}{2}
    % \right) \text{mlv}(x) -
    % \frac{\sigma_x ^ 2}{2} -
    % \frac{\sigma_x}{2} [
    %     1 - \text{mlv}(x)
    % ] (
    %     1 - 2\sigma_x
    % )\\
    % \text{sq}(x,\sigma_x) = 
    % \text{mlv}(x) + 
    % \frac{\sigma_x}{2}\left\{
    %     1 -
    %     \text{mlv}(x) -
    %     \frac{\sigma_x}{2} - 
    %     [1 - \text{mlv}(x)] (
    %         1 - 2\sigma_x
    %     )
    % \right\}\\
    % \text{sq}(x,\sigma_x) = 
    % \text{mlv}(x) + 
    % \frac{\sigma_x}{2}\left\{
    %     [1 - \text{mlv}(x)][1 - (1 - 2\sigma_x)]-
    %     \frac{\sigma_x}{2}
    % \right\}
    % \text{sq}(x,\sigma_x) = 
    % \text{mlv}(x) + 
    % \frac{\sigma_x}{2}\left\{
    %     (1 + 2\sigma_x)[1 - \text{mlv}(x)] -
    %     \frac{\sigma_x}{2}
    % \right\}, x \in [0,1]
    \text{sq}(\boldsymbol{x}) = 
    \text{mlv}(\boldsymbol{x}) + 
    \frac{\tilde{\sigma}_{x}}{2}\left\{
        (1 + 2\tilde{\sigma}_{x})[1 - \text{mlv}(\boldsymbol{x})] -
        \frac{\tilde{\sigma}_{x}}{2}
    \right\},\\
    \tilde{\sigma}_{x} = \frac{\sigma_{x}}{\max \sigma_{x}},\\
    % \tilde{\sigma}_{x} = \sigma_{x} / \max \sigma_{x},\\
    \boldsymbol{x} \in [0,1]^{m}\\
    % \text{sq}(\tilde{x},\sigma_{\tilde{x}}) = 
    % \text{mlv}({\tilde{x}}) + 
    % \frac{\sigma_{\tilde{x}}}{2}\left\{
    %     (1 + 2\sigma_{\tilde{x}})[1 - \text{mlv}({\tilde{x}})] -
    %     \frac{\sigma_{\tilde{x}}}{2}
    % \right\}
    % \frac{\sigma_x}{2} -
    % \frac{\sigma_x}{2} \text{mlv}(x) -
    % \frac{\sigma_x ^ 2}{2} -
    % \frac{\sigma_x}{2} [
    %     1 - \text{mlv}(x)
    % ] (
    %     1 - 2\sigma_x
    % )\\
    % 0.5 * dbl_sd +
    % (1 - 0.5 * dbl_sd) * dbl_mode +
    % -0.5 * dbl_sd * dbl_sd +
    % -0.5 * dbl_sd * (1 - dbl_mode) *
    % (1 - 2 * dbl_sd)
    \ddot{\tau}_{k,q} = 
    \text{edq}(\tau_{k}, \tau_{q}, c_{q}) = 
    \left\{
        1 + \exp[-
        \frac{
            \tau_{q}
            (\tau_{k} - \tau_{q})
        }{
            1 - c_{q}
        }
        ]
    \right\} ^ {-1}\\
    \textit{\ss}_{k,q} = 
    \ddot{s}_{k,q}
    \times
    \ddot{\tau}_{k,q} = 
    \text{eq}(s(\boldsymbol{a_k},\boldsymbol{a_q}), c_q)
    \times
    \text{edq}(\tau_{k}, \tau_{q}, c_{q})
\end{gather}

\end{document}